support for array_void_ptr

pulse/lib/steel/c/Steel.ST.C.Types.Array.fsti
@@ -168,14 +168,18 @@ val has_base_array_cell_equiv_to
 // ghost length of an array.
 
 [@@noextract_to "krml"] // primitive
-val array_ptr_gen ([@@@unused] t: Type0) : Tot Type0
+val array_void_ptr : Type0
+[@@noextract_to "krml"] // primitive
+let array_ptr_gen ([@@@unused] t: Type0) : Tot Type0 = array_void_ptr
 inline_for_extraction [@@noextract_to "krml"] // primitive
 let array_ptr (#t: Type) (td: typedef t) = array_ptr_gen t
 [@@noextract_to "krml"] // primitive
-val null_array_ptr (#t: Type) (td: typedef t) : Tot (array_ptr td)
+val null_array_void_ptr: array_void_ptr
+[@@noextract_to "krml"] // primitive
+let null_array_ptr (#t: Type) (td: typedef t) : Tot (array_ptr td) = null_array_void_ptr
 val g_array_ptr_is_null (#t: Type) (#td: typedef t) (a: array_ptr td) : Ghost bool
   (requires True)
-  (ensures (fun y -> y == true <==> a == null_array_ptr _))
+  (ensures (fun y -> y == true <==> a == null_array_ptr td))
 inline_for_extraction [@@noextract_to "krml"]
 let array_ref (#t: Type) (td: typedef t) = (a: array_ptr td { g_array_ptr_is_null a == false })
 
@@ -184,7 +188,7 @@ val array_ref_base_size_type (#t: Type) (#td: typedef t) (a: array_ref td) : GTo
 *)
 val array_ref_base_size (#t: Type) (#td: typedef t) (a: array_ptr td) : Ghost SZ.t
   (requires True)
-  (ensures (fun y -> SZ.v y == 0 <==> a == null_array_ptr _))
+  (ensures (fun y -> SZ.v y == 0 <==> a == null_array_ptr td))
 val has_array_ref_base (#t: Type) (#td: typedef t) (a: array_ref td) (#ty: Type) (r: ref (base_array0 ty td (array_ref_base_size a))) : GTot prop
 val has_array_ref_base_inj (#t: Type) (#td: typedef t) (a: array_ref td) (#ty: Type) (r1 r2: ref (base_array0 ty td (array_ref_base_size a))) : Lemma
   (requires (has_array_ref_base a r1 /\ has_array_ref_base a r2))
